Move various helper functions to Helpers.dfy

src/dafny/beacon/Helpers.dfy
@@ -15,6 +15,8 @@
 include "../utils/Eth2Types.dfy"
 include "../utils/MathHelpers.dfy"
 include "../utils/NativeTypes.dfy"
+include "../utils/SetHelpers.dfy"
+include "../utils/Helpers.dfy"
 
 include "../ssz/Constants.dfy"
 include "../ssz/Serialise.dfy"
@@ -23,7 +25,9 @@ include "BeaconChainTypes.dfy"
 include "Helpers.s.dfy"
 include "Helpers.p.dfy"
 include "attestations/AttestationsTypes.dfy"
+//include "attestations/AttestationsHelpers.dfy"
 include "validators/Validators.dfy"
+//include "validators/ValidatorHelpers.dfy"
 
 
 
@@ -36,6 +40,9 @@ module BeaconHelpers {
     import opened Eth2Types
     import opened MathHelpers
     import opened NativeTypes
+    import opened SetHelpers
+    import opened Helpers
+
 
     import opened Constants
     import opened SSZ
@@ -44,8 +51,12 @@ module BeaconHelpers {
     import opened BeaconHelperSpec
     import opened BeaconHelperProofs
     import opened AttestationsTypes
+    //import opened AttestationsHelpers
     import opened Validators
+    //import opened ValidatorHelpers
+
     
+
      /**
      * Extract a validator from a single deposit.
      *
@@ -769,7 +780,1515 @@ module BeaconHelpers {
         )
     } 
 
+
+    function method get_total_slashings(slashings: seq<Gwei>): Gwei
+    {
+        if |slashings| == 0 then 0 as Gwei
+        else 
+            assume slashings[0] as nat + get_total_slashings(slashings[1..]) as nat < 0x10000000000000000;
+            slashings[0] + get_total_slashings(slashings[1..])
+    }
+
+// Helpers - Rewards and penalties
+
+    function method integer_square_root(n:uint64) : uint64
+        requires n < 0xFFFFFFFFFFFFFFFF;
+        ensures power2(integer_square_root(n) as nat) <= n as nat;
+        //ensures !(exists x' {:trigger power(x' as nat,2)} :: x'>x && power(x' as nat,2) <= n as nat)
     
-       
+    function method get_base_reward(s: BeaconState, index: ValidatorIndex) : Gwei
+        requires index as int < |s.validators|
+        requires get_total_active_balance_full(s) < 0xFFFFFFFFFFFFFFFF 
+        requires integer_square_root(get_total_active_balance_full(s)) > 1
+        requires s.validators[index].effective_balance as int * BASE_REWARD_FACTOR as int / integer_square_root(get_total_active_balance_full(s)) as int / BASE_REWARDS_PER_EPOCH as int < 0x10000000000000000
+    {
+        var total_balance : Gwei := get_total_active_balance_full(s);
+        var effective_balance : Gwei := s.validators[index].effective_balance;
+
+        (EFFECTIVE_BALANCE_INCREMENT as int * BASE_REWARD_FACTOR as int / integer_square_root(total_balance) as int) as Gwei 
+    }
+
+    function method get_proposer_reward(state: BeaconState, attesting_index: ValidatorIndex): Gwei
+        requires attesting_index as int < |state.validators|
+        requires get_total_active_balance_full(state) < 0xFFFFFFFFFFFFFFFF 
+        requires integer_square_root(get_total_active_balance_full(state)) > 1
+        requires state.validators[attesting_index].effective_balance as int * BASE_REWARD_FACTOR as int / integer_square_root(get_total_active_balance_full(state)) as int / BASE_REWARDS_PER_EPOCH as int < 0x10000000000000000
+    {
+        (get_base_reward(state, attesting_index) / PROPOSER_REWARD_QUOTIENT) as Gwei  
+    }
+    
+    function method get_finality_delay(state: BeaconState): uint64
+        requires get_previous_epoch(state) >= state.finalised_checkpoint.epoch
+    {
+        get_previous_epoch(state) - state.finalised_checkpoint.epoch
+    }
+     
+    predicate method is_in_inactivity_leak(state: BeaconState)
+        requires get_previous_epoch(state) >= state.finalised_checkpoint.epoch
+    {
+        get_finality_delay(state) > MIN_EPOCHS_TO_INACTIVITY_PENALTY
+    }
+    
+    function method get_eligible_validator_indices(state: BeaconState): seq<ValidatorIndex>
+        ensures forall i :: 0 <= i < |get_eligible_validator_indices(state)|  
+            ==> get_eligible_validator_indices(state)[i] as nat < |state.validators|
+    {
+        var previous_epoch := get_previous_epoch(state);
+        get_eligible_validator_indices_helper(state.validators, previous_epoch)
+        //     return [
+        //         ValidatorIndex(index) for index, v in enumerate(state.validators)
+        //         if is_active_validator(v, previous_epoch) or (v.slashed and previous_epoch + 1 < v.withdrawable_epoch)
+        //     ]
+    }
+
+    function method get_eligible_validator_indices_helper(v: ListOfValidators, previous_epoch: Epoch): seq<ValidatorIndex>
+        ensures forall i :: 0 <= i < |get_eligible_validator_indices_helper(v, previous_epoch)|  
+            ==> get_eligible_validator_indices_helper(v, previous_epoch)[i] as nat < |v|
+    {
+        if |v| == 0 then []
+        else 
+            if is_active_validator(v[|v|-1], previous_epoch) || (v[|v|-1].slashed && (previous_epoch as int + 1 < v[|v|-1].withdrawable_epoch as int)) then
+                get_eligible_validator_indices_helper(v[..|v|-1], previous_epoch) + [(|v|-1) as ValidatorIndex]
+            else 
+                get_eligible_validator_indices_helper(v[..|v|-1], previous_epoch)
+    }
+
+    //datatype RewardsAndPenalties = rewardsAndPenalties(rewards: seq<Gwei>, penalties: seq<Gwei>)
+
+    /** Helper with shared logic for use by get source, target, and head deltas functions */
+
+    //Components of attestation deltas
+
+    // Return attester micro-rewards/penalties for source-vote for each validator.
+    function method get_source_deltas(s: BeaconState) : (seq<Gwei>,seq<Gwei>)
+        requires get_previous_epoch(s) >= s.finalised_checkpoint.epoch
+        requires get_total_active_balance_full(s) < 0xFFFFFFFFFFFFFFFF 
+        requires integer_square_root(get_total_active_balance_full(s)) > 1
+        requires EFFECTIVE_BALANCE_INCREMENT <= get_total_active_balance_full(s)
+
+        requires forall a :: a in get_matching_source_attestations(s, get_previous_epoch(s)) ==> a.data.index < get_committee_count_per_slot(s, compute_epoch_at_slot(a.data.slot)) <= TWO_UP_6
+        requires forall a :: a in get_matching_source_attestations(s, get_previous_epoch(s)) ==> TWO_UP_5 as nat <= |get_active_validator_indices(s.validators, compute_epoch_at_slot(a.data.slot))| <= TWO_UP_11 as nat * TWO_UP_11 as nat 
+        requires forall a :: a in get_matching_source_attestations(s, get_previous_epoch(s)) ==> 0 < |get_beacon_committee(s, a.data.slot, a.data.index)| == |a.aggregation_bits| <= MAX_VALIDATORS_PER_COMMITTEE as nat 
+    
+        ensures |get_source_deltas(s).0| == |get_source_deltas(s).1| == |s.validators|
+    {
+        var matching_source_attestations := get_matching_source_attestations(s, get_previous_epoch(s));
+
+        get_attestation_component_deltas(s, matching_source_attestations)
+    }
+
+    // Return attester micro-rewards/penalties for target-vote for each validator.
+    function method get_target_deltas(s: BeaconState) : (seq<Gwei>,seq<Gwei>)
+        requires get_previous_epoch(s) >= s.finalised_checkpoint.epoch
+        requires get_previous_epoch(s) as nat *  SLOTS_PER_EPOCH as nat  <  s.slot as nat
+        //requires s.slot - get_previous_epoch(s) *  SLOTS_PER_EPOCH <=  SLOTS_PER_HISTORICAL_ROOT  // equivalent to above requires
+
+        requires get_total_active_balance_full(s) < 0xFFFFFFFFFFFFFFFF 
+        requires integer_square_root(get_total_active_balance_full(s)) > 1
+        requires EFFECTIVE_BALANCE_INCREMENT <= get_total_active_balance_full(s)
+        requires 1 <= get_previous_epoch(s) <= get_current_epoch(s)
+
+        requires forall a :: a in get_matching_target_attestations(s, get_previous_epoch(s)) ==> a.data.index < get_committee_count_per_slot(s, compute_epoch_at_slot(a.data.slot)) <= TWO_UP_6
+        requires forall a :: a in get_matching_target_attestations(s, get_previous_epoch(s)) ==> TWO_UP_5 as nat <= |get_active_validator_indices(s.validators, compute_epoch_at_slot(a.data.slot))| <= TWO_UP_11 as nat * TWO_UP_11 as nat 
+        requires forall a :: a in get_matching_target_attestations(s, get_previous_epoch(s)) ==> 0 < |get_beacon_committee(s, a.data.slot, a.data.index)| == |a.aggregation_bits| <= MAX_VALIDATORS_PER_COMMITTEE as nat 
+    
+        ensures |get_target_deltas(s).0| == |get_target_deltas(s).1| == |s.validators|
+    {
+        var matching_target_attestations := get_matching_target_attestations(s, get_previous_epoch(s));
+
+        get_attestation_component_deltas(s, matching_target_attestations)
+    }
+
+
+    // def get_head_deltas(state: BeaconState) -> Tuple[Sequence[Gwei], Sequence[Gwei]]:
+    // """
+    // Return attester micro-rewards/penalties for head-vote for each validator.
+    // """
+    // matching_head_attestations = get_matching_head_attestations(state, get_previous_epoch(state))
+    // return get_attestation_component_deltas(state, matching_head_attestations)
+    function method get_head_deltas(s: BeaconState) : (seq<Gwei>,seq<Gwei>)
+        requires get_previous_epoch(s) >= s.finalised_checkpoint.epoch
+        requires get_previous_epoch(s) as nat *  SLOTS_PER_EPOCH as nat  <  s.slot as nat
+        //requires s.slot - get_previous_epoch(s) *  SLOTS_PER_EPOCH <=  SLOTS_PER_HISTORICAL_ROOT  // equivalent to above requires
+        requires get_total_active_balance_full(s) < 0xFFFFFFFFFFFFFFFF 
+        requires integer_square_root(get_total_active_balance_full(s)) > 1
+        requires EFFECTIVE_BALANCE_INCREMENT <= get_total_active_balance_full(s)
+        requires 1 <= get_previous_epoch(s) <= get_current_epoch(s)
+
+        requires forall a :: a in get_matching_head_attestations(s, get_previous_epoch(s)) ==> a.data.index < get_committee_count_per_slot(s, compute_epoch_at_slot(a.data.slot)) <= TWO_UP_6
+        requires forall a :: a in get_matching_head_attestations(s, get_previous_epoch(s)) ==> TWO_UP_5 as nat <= |get_active_validator_indices(s.validators, compute_epoch_at_slot(a.data.slot))| <= TWO_UP_11 as nat * TWO_UP_11 as nat 
+        requires forall a :: a in get_matching_head_attestations(s, get_previous_epoch(s)) ==> 0 < |get_beacon_committee(s, a.data.slot, a.data.index)| == |a.aggregation_bits| <= MAX_VALIDATORS_PER_COMMITTEE as nat 
+    
+        ensures |get_head_deltas(s).0| == |get_head_deltas(s).1| == |s.validators|
+    {
+        var matching_head_attestations := get_matching_head_attestations(s, get_previous_epoch(s));
+        get_attestation_component_deltas(s, matching_head_attestations)
+    }
+
+    // def get_inclusion_delay_deltas(state: BeaconState) -> Tuple[Sequence[Gwei], Sequence[Gwei]]:
+    // """
+    // Return proposer and inclusion delay micro-rewards/penalties for each validator.
+    // """
+    // rewards = [Gwei(0) for _ in range(len(state.validators))]
+    // matching_source_attestations = get_matching_source_attestations(state, get_previous_epoch(state))
+
+    // for index in get_unslashed_attesting_indices(state, matching_source_attestations):
+    //     attestation = min([
+    //         a for a in matching_source_attestations
+    //         if index in get_attesting_indices(state, a.data, a.aggregation_bits)
+    //     ], key=lambda a: a.inclusion_delay)
+    //     rewards[attestation.proposer_index] += get_proposer_reward(state, index)
+    //     max_attester_reward = Gwei(get_base_reward(state, index) - get_proposer_reward(state, index))
+    //     rewards[index] += Gwei(max_attester_reward // attestation.inclusion_delay)
+
+    // # No penalties associated with inclusion delay
+    // penalties = [Gwei(0) for _ in range(len(state.validators))]
+    // return rewards, penalties
+
+    function method get_inclusion_delay_deltas(s: BeaconState) : (seq<Gwei>,seq<Gwei>)
+        requires get_total_active_balance_full(s) < 0xFFFFFFFFFFFFFFFF 
+        requires integer_square_root(get_total_active_balance_full(s)) > 1
+
+        requires forall a :: a in get_matching_source_attestations(s, get_previous_epoch(s)) ==> a.data.index < get_committee_count_per_slot(s, compute_epoch_at_slot(a.data.slot)) <= TWO_UP_6
+        requires forall a :: a in get_matching_source_attestations(s, get_previous_epoch(s)) ==> TWO_UP_5 as nat <= |get_active_validator_indices(s.validators, compute_epoch_at_slot(a.data.slot))| <= TWO_UP_11 as nat * TWO_UP_11 as nat 
+        requires forall a :: a in get_matching_source_attestations(s, get_previous_epoch(s)) ==> 0 < |get_beacon_committee(s, a.data.slot, a.data.index)| == |a.aggregation_bits| <= MAX_VALIDATORS_PER_COMMITTEE as nat 
+        
+        ensures |get_inclusion_delay_deltas(s).0| == |get_inclusion_delay_deltas(s).1| == |s.validators|
+    {
+        var rewards : seq<Gwei> := timeSeq<Gwei>(0,|s.validators|);
+        var penalties : seq<Gwei> := timeSeq<Gwei>(0,|s.validators|);
+
+        var matching_source_attestations := get_matching_source_attestations(s, get_previous_epoch(s));
+        var unslashed_attesting_indices := get_unslashed_attesting_indices(s, matching_source_attestations);
+
+        // resolve the following assume at a later date i.e. look at the bound for effectBalance as part of the proof required
+        assume forall i :: i in unslashed_attesting_indices ==> s.validators[i].effective_balance as int * BASE_REWARD_FACTOR as int / integer_square_root(get_total_active_balance_full(s)) as int / BASE_REWARDS_PER_EPOCH as int < 0x10000000000000000;
+  
+        get_inclusion_delay_deltas_helper(s, unslashed_attesting_indices, matching_source_attestations, rewards, penalties)
+
+    }
+
+    function method get_inclusion_delay_deltas_helper(s: BeaconState, unslashed_attesting_indices: set<ValidatorIndex>, matching_source_attestations: seq<PendingAttestation>, rewards: seq<Gwei>, penalties: seq<Gwei>) : (seq<Gwei>,seq<Gwei>)
+        requires |rewards| == |penalties| == |s.validators|
+        requires forall i :: i in unslashed_attesting_indices ==> i as int < |s.validators|
+        requires get_total_active_balance_full(s) < 0xFFFFFFFFFFFFFFFF 
+        requires integer_square_root(get_total_active_balance_full(s)) > 1
+        requires forall i :: i in unslashed_attesting_indices ==> 
+                s.validators[i as nat].effective_balance as int * BASE_REWARD_FACTOR as int / integer_square_root(get_total_active_balance_full(s)) as int / BASE_REWARDS_PER_EPOCH as int < 0x10000000000000000
+
+        ensures |get_inclusion_delay_deltas_helper(s, unslashed_attesting_indices, matching_source_attestations, rewards, penalties).0| == |rewards| == |s.validators|
+        ensures |get_inclusion_delay_deltas_helper(s, unslashed_attesting_indices, matching_source_attestations, rewards, penalties).1| == |penalties| == |s.validators|
+    
+    {
+        if unslashed_attesting_indices == {} then (rewards, penalties)
+        else
+            var index := PickIndex(unslashed_attesting_indices);
+            var attestation := get_min_attestation(matching_source_attestations, index);
+            assume attestation.proposer_index as nat < |rewards|;
+            assume (rewards[attestation.proposer_index as nat] as nat + get_proposer_reward(s, index) as nat) < 0x10000000000000000; 
+            var rewards' := rewards[attestation.proposer_index as nat := (rewards[attestation.proposer_index as nat] as nat + get_proposer_reward(s, index) as nat) as Gwei];
+            var penalties' := penalties;
+            
+            assume get_base_reward(s, index) > get_proposer_reward(s, index);
+            // or set to 0
+            var max_attester_reward := get_base_reward(s, index) - get_proposer_reward(s, index);
+            assume attestation.inclusion_delay > 0;
+            assume (rewards'[index as nat] as nat + max_attester_reward as nat / attestation.inclusion_delay as nat) < 0x10000000000000000;
+
+            assert |rewards'| == |rewards|;
+            assert |penalties'| == |penalties|;
+            get_inclusion_delay_deltas_helper(s, unslashed_attesting_indices - {index}, matching_source_attestations, rewards'[index as nat := (rewards'[index as nat] as nat
+                                            + max_attester_reward as nat / attestation.inclusion_delay as nat) as Gwei], penalties)
+
+    }
+
+    function method get_min_attestation(sa : seq<PendingAttestation>, index: ValidatorIndex) : PendingAttestation
+        
+
+    // def get_inactivity_penalty_deltas(state: BeaconState) -> Tuple[Sequence[Gwei], Sequence[Gwei]]:
+    // """
+    
+    // """
+    // penalties = [Gwei(0) for _ in range(len(state.validators))]
+    // if is_in_inactivity_leak(state):
+    //     matching_target_attestations = get_matching_target_attestations(state, get_previous_epoch(state))
+    //     matching_target_attesting_indices = get_unslashed_attesting_indices(state, matching_target_attestations)
+    //     for index in get_eligible_validator_indices(state):
+    //         # If validator is performing optimally this cancels all rewards for a neutral balance
+    //         base_reward = get_base_reward(state, index)
+    //         penalties[index] += Gwei(BASE_REWARDS_PER_EPOCH * base_reward - get_proposer_reward(state, index))
+    //         if index not in matching_target_attesting_indices:
+    //             effective_balance = state.validators[index].effective_balance
+    //             penalties[index] += Gwei(effective_balance * get_finality_delay(state) // INACTIVITY_PENALTY_QUOTIENT)
+
+    // # No rewards associated with inactivity penalties
+    // rewards = [Gwei(0) for _ in range(len(state.validators))]
+    // return rewards, penalties
+
+    // Return inactivity reward/penalty deltas for each validator.
+    function method get_inactivity_penalty_deltas(s: BeaconState) : (seq<Gwei>,seq<Gwei>)
+        requires get_previous_epoch(s) >= s.finalised_checkpoint.epoch
+        requires get_previous_epoch(s) as nat *  SLOTS_PER_EPOCH as nat  <  s.slot as nat
+        requires s.slot - get_previous_epoch(s) *  SLOTS_PER_EPOCH <=  SLOTS_PER_HISTORICAL_ROOT 
+        requires 1 <= get_previous_epoch(s) <= get_current_epoch(s)
+        requires get_total_active_balance_full(s) < 0xFFFFFFFFFFFFFFFF 
+        requires integer_square_root(get_total_active_balance_full(s)) > 1
+
+        requires forall a :: a in get_matching_target_attestations(s, get_previous_epoch(s)) ==> a.data.index < get_committee_count_per_slot(s, compute_epoch_at_slot(a.data.slot)) <= TWO_UP_6
+        requires forall a :: a in get_matching_target_attestations(s, get_previous_epoch(s)) ==> TWO_UP_5 as nat <= |get_active_validator_indices(s.validators, compute_epoch_at_slot(a.data.slot))| <= TWO_UP_11 as nat * TWO_UP_11 as nat 
+        requires forall a :: a in get_matching_target_attestations(s, get_previous_epoch(s)) ==> 0 < |get_beacon_committee(s, a.data.slot, a.data.index)| == |a.aggregation_bits| <= MAX_VALIDATORS_PER_COMMITTEE as nat 
+        
+        ensures |get_inactivity_penalty_deltas(s).0| == |get_inactivity_penalty_deltas(s).1| == |s.validators|
+    {
+        var rewards : seq<Gwei> := timeSeq<Gwei>(0,|s.validators|);
+        var penalties : seq<Gwei> := timeSeq<Gwei>(0,|s.validators|);
+
+        if (is_in_inactivity_leak(s)) then
+            var matching_target_attestations := get_matching_target_attestations(s, get_previous_epoch(s));
+            var matching_target_attesting_indices := get_unslashed_attesting_indices(s, matching_target_attestations);
+            var eligible_validator_indices := get_eligible_validator_indices(s);
+            assert forall i :: 0 <= i < |eligible_validator_indices| ==> eligible_validator_indices[i] as nat < |s.validators|;
+        
+            assume forall i :: 0 <= i < |eligible_validator_indices| ==> s.validators[eligible_validator_indices[i] as nat].effective_balance as int * BASE_REWARD_FACTOR as int / integer_square_root(get_total_active_balance_full(s)) as int / BASE_REWARDS_PER_EPOCH as int < 0x10000000000000000;
+   
+            get_inactivity_penalty_deltas_helper(s, eligible_validator_indices, matching_target_attesting_indices, rewards, penalties)
+        else    
+            (rewards,penalties)
+        
+    }
+
+    function method get_inactivity_penalty_deltas_helper(s: BeaconState, 
+                                                    eligible_indices: seq<ValidatorIndex>, 
+                                                    target_indices: set<ValidatorIndex>,
+                                                    rewards: seq<Gwei>,
+                                                    penalties: seq<Gwei>)  
+                                                : (seq<Gwei>,seq<Gwei>)
+        requires |rewards| == |penalties| == |s.validators|
+        requires forall i :: 0 <= i < |eligible_indices| ==> eligible_indices[i] as nat < |s.validators|
+        requires get_total_active_balance_full(s) < 0xFFFFFFFFFFFFFFFF 
+        requires integer_square_root(get_total_active_balance_full(s)) > 1
+        requires forall i :: 0 <= i < |eligible_indices| ==> s.validators[eligible_indices[i] as nat].effective_balance as int * BASE_REWARD_FACTOR as int / integer_square_root(get_total_active_balance_full(s)) as int / BASE_REWARDS_PER_EPOCH as int < 0x10000000000000000
+        requires get_previous_epoch(s) >= s.finalised_checkpoint.epoch
+
+         ensures |get_inactivity_penalty_deltas_helper(s, eligible_indices, target_indices, rewards, penalties).0| == |rewards| == |s.validators|
+        ensures |get_inactivity_penalty_deltas_helper(s, eligible_indices, target_indices, rewards, penalties).1| == |penalties| == |s.validators|
+    {
+        if |eligible_indices| == 0 then (rewards, penalties)
+        else
+            var base_reward := get_base_reward(s,eligible_indices[0]);
+            var first_part_of_penalty := (BASE_REWARDS_PER_EPOCH * base_reward - get_proposer_reward(s, eligible_indices[0])) as Gwei;
+
+            var rewards' := rewards;
+            assert |rewards'| == |rewards|;
+            
+
+            if eligible_indices[0] !in target_indices then
+                var effective_balance := s.validators[eligible_indices[0] as nat].effective_balance;
+                assume INACTIVITY_PENALTY_QUOTIENT as nat > 0;
+                assume (effective_balance as nat * get_finality_delay(s) as nat / INACTIVITY_PENALTY_QUOTIENT as nat) < 0x10000000000000000;
+                var second_part_of_penalty := (effective_balance as nat * get_finality_delay(s) as nat / INACTIVITY_PENALTY_QUOTIENT as nat) as Gwei;
+                
+                assume (penalties[eligible_indices[0] as nat] as nat + first_part_of_penalty as nat + second_part_of_penalty as nat) < 0x10000000000000000;
+                var penalties' := penalties[eligible_indices[0] as nat := (penalties[eligible_indices[0] as nat] as nat + first_part_of_penalty as nat + second_part_of_penalty as nat) as Gwei];
+                assert |penalties'| == |penalties|;
+
+                get_inactivity_penalty_deltas_helper(s, eligible_indices[1..], target_indices, rewards', penalties')
+            else
+                assume penalties[eligible_indices[0] as nat] as nat + first_part_of_penalty as nat < 0x10000000000000000;
+                var penalties' := penalties[eligible_indices[0] as nat := (penalties[eligible_indices[0] as nat] as nat + first_part_of_penalty as nat) as Gwei];
+                assert |penalties'| == |penalties|;
+                get_inactivity_penalty_deltas_helper(s, eligible_indices[1..], target_indices, rewards', penalties')
+            
+    }
+
+
+    
+    // Helper with shared logic for use by get source, target, and head deltas functions
+    function method get_attestation_component_deltas(s: BeaconState, attestations: seq<PendingAttestation>) : (seq<Gwei>,seq<Gwei>)
+        requires get_previous_epoch(s) >= s.finalised_checkpoint.epoch
+        requires get_total_active_balance_full(s) < 0xFFFFFFFFFFFFFFFF 
+        requires integer_square_root(get_total_active_balance_full(s)) > 1
+        requires EFFECTIVE_BALANCE_INCREMENT <= get_total_active_balance_full(s) 
+
+        requires forall a :: a in attestations ==> a.data.index < get_committee_count_per_slot(s, compute_epoch_at_slot(a.data.slot)) <= TWO_UP_6
+        requires forall a :: a in attestations ==> TWO_UP_5 as nat <= |get_active_validator_indices(s.validators, compute_epoch_at_slot(a.data.slot))| <= TWO_UP_11 as nat * TWO_UP_11 as nat 
+        requires forall a :: a in attestations ==> 0 < |get_beacon_committee(s, a.data.slot, a.data.index)| == |a.aggregation_bits| <= MAX_VALIDATORS_PER_COMMITTEE as nat 
+
+        ensures |get_attestation_component_deltas(s, attestations).0| == |get_attestation_component_deltas(s, attestations).1| == |s.validators|
+        
+    {
+        var rewards : seq<Gwei> := timeSeq<Gwei>(0,|s.validators|);
+        var penalties : seq<Gwei> := timeSeq<Gwei>(0,|s.validators|);
+        var total_balance := get_total_active_balance_full(s);
+        var unslashed_attesting_indices := get_unslashed_attesting_indices(s, attestations);
+        var attesting_balance := get_total_balance(s, unslashed_attesting_indices);
+        var indices := get_eligible_validator_indices(s);
+
+        assert forall i :: 0 <= i < |indices| ==> indices[i] as nat < |s.validators|;
+
+        // resolve the following assume at a later date i.e. look at the bound for effectBalance as part of the proof required
+        assume forall i :: 0 <= i < |indices| ==> s.validators[indices[i]].effective_balance as int * BASE_REWARD_FACTOR as int / integer_square_root(get_total_active_balance_full(s)) as int / BASE_REWARDS_PER_EPOCH as int < 0x10000000000000000;
+  
+        
+        get_attestation_component_deltas_helper(s, indices, total_balance, unslashed_attesting_indices, attesting_balance, rewards, penalties)
+        
+    }
+
+    function method get_attestation_component_deltas_helper(s: BeaconState, 
+                                                    indices: seq<ValidatorIndex>, 
+                                                    total_balance: Gwei,
+                                                    unslashed_attesting_indices: set<ValidatorIndex>,
+                                                    attesting_balance: Gwei,
+                                                    rewards: seq<Gwei>,
+                                                    penalties: seq<Gwei>)  
+                                                : (seq<Gwei>,seq<Gwei>)
+        requires |rewards| == |penalties| == |s.validators|
+        requires EFFECTIVE_BALANCE_INCREMENT <= total_balance 
+        requires get_previous_epoch(s) >= s.finalised_checkpoint.epoch
+        requires forall i :: 0 <= i < |indices| ==> indices[i] as nat < |s.validators|
+        requires get_total_active_balance_full(s) < 0xFFFFFFFFFFFFFFFF 
+        requires integer_square_root(get_total_active_balance_full(s)) > 1
+        requires forall i :: 0 <= i < |indices| ==> s.validators[indices[i]].effective_balance as int * BASE_REWARD_FACTOR as int / integer_square_root(get_total_active_balance_full(s)) as int / BASE_REWARDS_PER_EPOCH as int < 0x10000000000000000
+     
+        ensures |get_attestation_component_deltas_helper(s, indices, total_balance, unslashed_attesting_indices, attesting_balance, rewards, penalties).0| == |rewards| == |s.validators|
+        ensures |get_attestation_component_deltas_helper(s, indices, total_balance, unslashed_attesting_indices, attesting_balance, rewards, penalties).1| == |penalties| == |s.validators|
+    {
+        if |indices| == 0 then (rewards, penalties)
+        else
+            var index := indices[0];
+            assert index as nat < |s.validators|;
+            assert integer_square_root(get_total_active_balance_full(s)) > 1;
+            assert s.validators[index].effective_balance as int * BASE_REWARD_FACTOR as int / integer_square_root(get_total_active_balance_full(s)) as int / BASE_REWARDS_PER_EPOCH as int < 0x10000000000000000;
+
+            if index in unslashed_attesting_indices then
+                var increment := EFFECTIVE_BALANCE_INCREMENT;
+                var rewards_numerator :=  get_base_reward(s, index) as nat * (attesting_balance as nat / increment as nat); // this is moved above the else branch to faciliate the related assume statement
+
+                assert (total_balance as nat / increment as nat) >= 1;
+                // resolve the following assume at a later date i.e. look at the bounds for each component
+                assume rewards_numerator > 0;
+                assume rewards[index as nat] as nat + get_base_reward(s, index) as nat < 0x10000000000000000;
+                assume rewards[index as nat] as nat + rewards_numerator / (total_balance as nat / increment as nat) < 0x10000000000000000;
+                
+                if is_in_inactivity_leak(s) then   
+                    //(rewards[indices[0] := rewards[indices[0]] + get_base_reward(s, indices[0])], penalties)
+                    get_attestation_component_deltas_helper(s, indices[1..], total_balance, unslashed_attesting_indices, attesting_balance, rewards[index as nat := (rewards[index as nat] as nat + get_base_reward(s, index) as nat) as Gwei], penalties)
+                else
+                    //  var rewards_numerator :=  get_base_reward(s, index) * (attesting_balance / increment); 
+                    //(rewards[indices[0] := rewards[indices[0]] + rewards_numerator / (total_balance / increment)], penalties)
+                    get_attestation_component_deltas_helper(s, indices[1..], total_balance, unslashed_attesting_indices, attesting_balance, rewards[index as nat := (rewards[index as nat] as nat + rewards_numerator / (total_balance as nat / increment as nat)) as Gwei], penalties)
+            else
+                // resolve the following assume at a later date i.e. look at the bounds for each component
+                assume penalties[index as nat] as nat + get_base_reward(s, index) as nat < 0x10000000000000000;
+
+                //(rewards, penalties[indices[0] := penalties[indices[0]] + get_base_reward(s, indices[0])])
+                get_attestation_component_deltas_helper(s, indices[1..], total_balance, unslashed_attesting_indices, attesting_balance, rewards, penalties[index as nat := (penalties[index as nat] as nat + get_base_reward(s, index) as nat) as Gwei])
+
+    }
+    
+    
+    // def get_attestation_deltas(state: BeaconState) -> Tuple[Sequence[Gwei], Sequence[Gwei]]:
+    // """
+    // Return attestation reward/penalty deltas for each validator.
+    // """
+    // source_rewards, source_penalties = get_source_deltas(state)
+    // target_rewards, target_penalties = get_target_deltas(state)
+    // head_rewards, head_penalties = get_head_deltas(state)
+    // inclusion_delay_rewards, _ = get_inclusion_delay_deltas(state)
+    // _, inactivity_penalties = get_inactivity_penalty_deltas(state)
+
+    // rewards = [
+    //     source_rewards[i] + target_rewards[i] + head_rewards[i] + inclusion_delay_rewards[i]
+    //     for i in range(len(state.validators))
+    // ]
+
+    // penalties = [
+    //     source_penalties[i] + target_penalties[i] + head_penalties[i] + inactivity_penalties[i]
+    //     for i in range(len(state.validators))
+    // ]
+
+    // return rewards, penalties
+    function method get_attestation_deltas(s: BeaconState) : (seq<Gwei>, seq<Gwei>)
+        //requires get_previous_epoch(s) >= s.finalised_checkpoint.epoch
+        //requires integer_square_root(get_total_active_balance_full(s)) > 1
+        //requires get_total_active_balance_full(s) > 1
+        //requires EFFECTIVE_BALANCE_INCREMENT <= get_total_active_balance_full(s)
+
+        //requires get_previous_epoch(s) as nat *  SLOTS_PER_EPOCH as nat  <  s.slot as nat
+        requires 1 <= get_previous_epoch(s) //<= get_current_epoch(s)
+        // i.e. this means it isn't applicable to the GENESIS_EPOCH
+
+        requires forall a :: a in s.previous_epoch_attestations ==> a.data.index < get_committee_count_per_slot(s, compute_epoch_at_slot(a.data.slot)) <= TWO_UP_6
+        requires forall a :: a in s.previous_epoch_attestations ==> TWO_UP_5 as nat <= |get_active_validator_indices(s.validators, compute_epoch_at_slot(a.data.slot))| <= TWO_UP_11 as nat * TWO_UP_11 as nat 
+        requires forall a :: a in s.previous_epoch_attestations ==> 0 < |get_beacon_committee(s, a.data.slot, a.data.index)| == |a.aggregation_bits| <= MAX_VALIDATORS_PER_COMMITTEE as nat 
+
+
+        // requires forall a :: a in get_matching_source_attestations(s, get_previous_epoch(s)) ==> a.data.index < get_committee_count_per_slot(s, compute_epoch_at_slot(a.data.slot)) <= TWO_UP_6
+        // requires forall a :: a in get_matching_source_attestations(s, get_previous_epoch(s)) ==> TWO_UP_5 as nat <= |get_active_validator_indices(s.validators, compute_epoch_at_slot(a.data.slot))| <= TWO_UP_11 as nat * TWO_UP_11 as nat 
+        // requires forall a :: a in get_matching_source_attestations(s, get_previous_epoch(s)) ==> 0 < |get_beacon_committee(s, a.data.slot, a.data.index)| == |a.aggregation_bits| <= MAX_VALIDATORS_PER_COMMITTEE as nat 
+    
+        // requires forall a :: a in get_matching_target_attestations(s, get_previous_epoch(s)) ==> a.data.index < get_committee_count_per_slot(s, compute_epoch_at_slot(a.data.slot)) <= TWO_UP_6
+        // requires forall a :: a in get_matching_target_attestations(s, get_previous_epoch(s)) ==> TWO_UP_5 as nat <= |get_active_validator_indices(s.validators, compute_epoch_at_slot(a.data.slot))| <= TWO_UP_11 as nat * TWO_UP_11 as nat 
+        // requires forall a :: a in get_matching_target_attestations(s, get_previous_epoch(s)) ==> 0 < |get_beacon_committee(s, a.data.slot, a.data.index)| == |a.aggregation_bits| <= MAX_VALIDATORS_PER_COMMITTEE as nat 
+    
+        // requires forall a :: a in get_matching_head_attestations(s, get_previous_epoch(s)) ==> a.data.index < get_committee_count_per_slot(s, compute_epoch_at_slot(a.data.slot)) <= TWO_UP_6
+        // requires forall a :: a in get_matching_head_attestations(s, get_previous_epoch(s)) ==> TWO_UP_5 as nat <= |get_active_validator_indices(s.validators, compute_epoch_at_slot(a.data.slot))| <= TWO_UP_11 as nat * TWO_UP_11 as nat 
+        // requires forall a :: a in get_matching_head_attestations(s, get_previous_epoch(s)) ==> 0 < |get_beacon_committee(s, a.data.slot, a.data.index)| == |a.aggregation_bits| <= MAX_VALIDATORS_PER_COMMITTEE as nat 
+    
+        ensures |get_attestation_deltas(s).0| == |get_attestation_deltas(s).1| == |s.validators|
+    {
+        //assert forall a :: a in get_matching_source_attestations(s, get_previous_epoch(s)) ==> a in s.previous_epoch_attestations;
+        // assert forall a :: a in get_matching_source_attestations(s, get_previous_epoch(s)) ==> a.data.index < get_committee_count_per_slot(s, compute_epoch_at_slot(a.data.slot)) <= TWO_UP_6;
+        // assert forall a :: a in get_matching_source_attestations(s, get_previous_epoch(s)) ==> TWO_UP_5 as nat <= |get_active_validator_indices(s.validators, compute_epoch_at_slot(a.data.slot))| <= TWO_UP_11 as nat * TWO_UP_11 as nat; 
+        // assert forall a :: a in get_matching_source_attestations(s, get_previous_epoch(s)) ==> 0 < |get_beacon_committee(s, a.data.slot, a.data.index)| == |a.aggregation_bits| <= MAX_VALIDATORS_PER_COMMITTEE as nat ;
+    
+        // assert forall a :: a in get_matching_target_attestations(s, get_previous_epoch(s)) ==> a.data.index < get_committee_count_per_slot(s, compute_epoch_at_slot(a.data.slot)) <= TWO_UP_6;
+        // assert forall a :: a in get_matching_target_attestations(s, get_previous_epoch(s)) ==> TWO_UP_5 as nat <= |get_active_validator_indices(s.validators, compute_epoch_at_slot(a.data.slot))| <= TWO_UP_11 as nat * TWO_UP_11 as nat ;
+        // assert forall a :: a in get_matching_target_attestations(s, get_previous_epoch(s)) ==> 0 < |get_beacon_committee(s, a.data.slot, a.data.index)| == |a.aggregation_bits| <= MAX_VALIDATORS_PER_COMMITTEE as nat; 
+    
+        // assert forall a :: a in get_matching_head_attestations(s, get_previous_epoch(s)) ==> a.data.index < get_committee_count_per_slot(s, compute_epoch_at_slot(a.data.slot)) <= TWO_UP_6;
+        // assert forall a :: a in get_matching_head_attestations(s, get_previous_epoch(s)) ==> TWO_UP_5 as nat <= |get_active_validator_indices(s.validators, compute_epoch_at_slot(a.data.slot))| <= TWO_UP_11 as nat * TWO_UP_11 as nat ;
+        // assert forall a :: a in get_matching_head_attestations(s, get_previous_epoch(s)) ==> 0 < |get_beacon_committee(s, a.data.slot, a.data.index)| == |a.aggregation_bits| <= MAX_VALIDATORS_PER_COMMITTEE as nat ;
+    
+        
+        var rewards : seq<Gwei> := timeSeq<Gwei>(0,|s.validators|);
+        var penalties : seq<Gwei> := timeSeq<Gwei>(0,|s.validators|);
+        
+        assume get_previous_epoch(s) >= s.finalised_checkpoint.epoch;
+        assert EFFECTIVE_BALANCE_INCREMENT <= get_total_active_balance_full(s);
+
+        assume get_total_active_balance_full(s) < 0xFFFFFFFFFFFFFFFF;
+        assume integer_square_root(get_total_active_balance_full(s)) > 1; // ie as EFFECTIVE_BALANCE_INCREMENT <= get_total_active_balance_full(s)
+        assert get_previous_epoch(s) as nat *  SLOTS_PER_EPOCH as nat  <  s.slot as nat;
+        
+        var (sr, sp) := get_source_deltas(s);
+        var (tr, tp) := get_target_deltas(s);
+        var (hr, hp) := get_head_deltas(s);
+        var (ddr, ddp) := get_inclusion_delay_deltas(s);
+        var (pdr, pdp) := get_inactivity_penalty_deltas(s);
+
+        assert |sr| == |tr| == |hr| == |ddr| == |pdr| == |s.validators|;
+        assert |sp| == |tp| == |hp| == |ddp| == |pdp| == |s.validators|;
+
+        (get_attestation_deltas_helper_sum_rewards(sr, tr, hr, ddr, pdr, rewards),
+         get_attestation_deltas_helper_sum_penalties(sp, tp, hp, ddp, pdp, penalties))
+
+    }
+
+    function method get_attestation_deltas_helper_sum_rewards(sr: seq<Gwei>, tr: seq<Gwei>, hr: seq<Gwei>, ddr: seq<Gwei>, pdr: seq<Gwei>, rewards: seq<Gwei>) : seq<Gwei>
+        requires |sr| == |tr| == |hr| == |ddr| == |pdr| <= |rewards|
+        ensures |get_attestation_deltas_helper_sum_rewards(sr, tr, hr, ddr, pdr, rewards)| == |rewards|
+    {
+        if |sr| == 0 then rewards
+        else    
+            assume rewards[0] as nat + sr[0] as nat + tr[0] as nat + hr[0] as nat + ddr[0] as nat + pdr[0] as nat < 0x10000000000000000;
+            get_attestation_deltas_helper_sum_rewards(sr[1..], tr[1..], hr[1..], ddr[1..], pdr[1..], rewards[0 := rewards[0] + sr[0] + tr[0] + hr[0] + ddr[0] + pdr[0]])
+    }
+
+    function method get_attestation_deltas_helper_sum_penalties(sp: seq<Gwei>, tp: seq<Gwei>, hp: seq<Gwei>, ddp: seq<Gwei>, pdp: seq<Gwei>, penalties: seq<Gwei>) : seq<Gwei>
+        requires |sp| == |tp| == |hp| == |ddp| == |pdp| <= |penalties|
+        ensures |get_attestation_deltas_helper_sum_penalties(sp, tp, hp, ddp, pdp, penalties)| == |penalties|
+    {
+        if |sp| == 0 then penalties
+        else    
+            assume penalties[0] as nat + sp[0] as nat + tp[0] as nat + hp[0] as nat + ddp[0] as nat + pdp[0] as nat  < 0x10000000000000000;
+            get_attestation_deltas_helper_sum_penalties(sp[1..], tp[1..], hp[1..], ddp[1..], pdp[1..], penalties[0 := penalties[0] + sp[0] + tp[0] + hp[0] + ddp[0] + pdp[0]])
+    }
+
+
+    
+
+    /**
+     *  Check if there is at least one active validator.
+     *
+     *  @param      s   A beacon state.
+     *  @returns        True if 
+     *                  |get_active_validator_indices(s.validators, get_current_epoch(s))| > 0,
+     *                  otherwise False.
+     */
+    predicate minimumActiveValidators(s: BeaconState)
+    {
+        |get_active_validator_indices(s.validators, get_current_epoch(s))| > 0
+    }
+    
+    /** initiate_validator_exit
+     *  
+     *  Initiate the exit of the validator with index ``index``.
+     *
+     */
+    function method initiate_validator_exit(s: BeaconState, index: ValidatorIndex) : BeaconState
+        requires |s.validators| == |s.balances|
+        requires index as int < |s.validators| 
+        //requires s.validators[index].exitEpoch == FAR_FUTURE_EPOCH
+
+        ensures |s.validators| == |initiate_validator_exit(s,index).validators|
+        ensures |initiate_validator_exit(s,index).validators| == |initiate_validator_exit(s,index).balances|
+        ensures initiate_validator_exit(s,index).validators[index].exitEpoch > get_current_epoch(s) + MAX_SEED_LOOKAHEAD
+                || initiate_validator_exit(s,index).validators[index].exitEpoch == s.validators[index].exitEpoch
+        ensures forall i :: (0 <= i < |s.validators|) && (i != index as int) ==> 
+                initiate_validator_exit(s,index).validators[i].exitEpoch == s.validators[i].exitEpoch
+        ensures initiate_validator_exit(s,index).validators[index].exitEpoch < FAR_FUTURE_EPOCH
+    {
+        // # Return if validator already initiated exit
+        // validator = state.validators[index]
+        if s.validators[index].exitEpoch != FAR_FUTURE_EPOCH then
+            s
+        else 
+        //     return
+        //assert s.validators[index].exitEpoch == FAR_FUTURE_EPOCH;
+        
+        // # Compute exit queue epoch
+        // exit_epochs = [v.exit_epoch for v in state.validators if v.exit_epoch != FAR_FUTURE_EPOCH]
+        var exit_epochs := get_exit_epochs(s.validators);
+        
+        // exit_queue_epoch = max(exit_epochs + [compute_activation_exit_epoch(get_current_epoch(state))])
+        var exit_queue_epoch := max_epoch(exit_epochs + [compute_activation_exit_epoch(get_current_epoch(s))]);
+
+        assert compute_activation_exit_epoch(get_current_epoch(s)) > get_current_epoch(s) + MAX_SEED_LOOKAHEAD;
+        assert compute_activation_exit_epoch(get_current_epoch(s)) in exit_epochs + [compute_activation_exit_epoch(get_current_epoch(s))];
+        assert max_epoch(exit_epochs + [compute_activation_exit_epoch(get_current_epoch(s))]) >= compute_activation_exit_epoch(get_current_epoch(s));
+        assert exit_queue_epoch > get_current_epoch(s) + MAX_SEED_LOOKAHEAD;
+
+        // exit_queue_churn = len([v for v in state.validators if v.exit_epoch == exit_queue_epoch])
+        var exit_queue_churn := |get_queue_churn(s.validators, exit_queue_epoch)|;
+        var validator_churn_limit := get_validator_churn_limit(s);
+
+        // if exit_queue_churn >= get_validator_churn_limit(state):
+        //     exit_queue_epoch += Epoch(1)
+
+        // # Set validator exit epoch and withdrawable epoch
+        // validator.exit_epoch = exit_queue_epoch
+        // validator.withdrawable_epoch = Epoch(validator.exit_epoch + MIN_VALIDATOR_WITHDRAWABILITY_DELAY)
+
+        assume exit_queue_epoch as int + 1 + MIN_VALIDATOR_WITHDRAWABILITY_DELAY as nat < 0x10000000000000000; 
+
+        if exit_queue_churn  >= get_validator_churn_limit(s) as nat then 
+            s.(validators := s.validators[index as int := s.validators[index].(exitEpoch := exit_queue_epoch + 1 as Epoch,
+                                                            withdrawable_epoch := (exit_queue_epoch as nat + 1 + MIN_VALIDATOR_WITHDRAWABILITY_DELAY as nat) as Epoch)])
+        else
+            s.(validators := s.validators[index as int := s.validators[index].(exitEpoch := exit_queue_epoch,
+                                                            withdrawable_epoch := (exit_queue_epoch as nat + MIN_VALIDATOR_WITHDRAWABILITY_DELAY as nat) as Epoch)])
+    }
+
+
+        /** slash_validator
+     *  
+     *  Slash the validator with index ``slashed_index``.
+     */
+    function method slash_validator(s: BeaconState, slashed_index: ValidatorIndex, whistleblower_index: ValidatorIndex): BeaconState
+        requires slashed_index as int < |s.validators| 
+        requires whistleblower_index as int < |s.validators| 
+        requires |s.validators| == |s.balances|
+        //requires s.validators[slashed_index].exitEpoch == FAR_FUTURE_EPOCH
+        requires |get_active_validator_indices(s.validators, get_current_epoch(s))| > 0
+        //ensures |get_active_validator_indices(slash_validator(s,slashed_index,whistleblower_index).validators, get_current_epoch(s))| > 0
+        ensures slash_validator(s, slashed_index, whistleblower_index).slot == s.slot
+    {
+        var epoch : Epoch := get_current_epoch(s);
+        var proposer_index := get_beacon_proposer_index(s);
+
+        var s' := initiate_validator_exit(s, slashed_index); // only validator exitEpoch & withdrawable_epoch fields possibly changed
+
+        assert |s.balances| == |s'.balances|;
+        assert |s'.balances| == |s'.validators|;
+        assert get_current_epoch(s) == get_current_epoch(s');
+        
+        //assert initiate_validator_exit(s,slashed_index).validators[slashed_index].exitEpoch > get_current_epoch(s) + MAX_SEED_LOOKAHEAD;
+        assert forall i :: (0 <= i < |s.validators|) && (i != slashed_index as int) ==> 
+                initiate_validator_exit(s,slashed_index).validators[i].exitEpoch == s.validators[i].exitEpoch;
+        
+        //assert s'.validators[slashed_index].exitEpoch > get_current_epoch(s) + MAX_SEED_LOOKAHEAD;
+        assert forall i :: (0 <= i < |s.validators|) && (i != slashed_index as int) ==> 
+                s'.validators[i].exitEpoch == s.validators[i].exitEpoch;
+        
+        assert forall i :: (0 <= i < |s'.validators|) ==> 
+                is_active_validator(s.validators[i], get_current_epoch(s)) == is_active_validator(s'.validators[i], get_current_epoch(s'));
+
+        initiateValidatorExitPreservesActivateValidators(s.validators, s'.validators,  get_current_epoch(s'));
+        assert get_active_validator_indices(s'.validators, get_current_epoch(s')) == get_active_validator_indices(s.validators, get_current_epoch(s));
+        assert |get_active_validator_indices(s'.validators, get_current_epoch(s'))| > 0;
+        
+        // NOTE:    steps reordered to suit Dafny function method output
+        //          order irrelevant as 'Apply proposer and whistleblower rewards' relies only on s'.validators[slashed_index].effective_balance
+
+        // # Apply proposer and whistleblower rewards
+        
+        // if whistleblower_index is None:
+        //     whistleblower_index = proposer_index
+        // Note: 'None' is not available in Dafny and so functions that call slash_validator will have this parameter set to proposer_index
+        
+        
+        // NOTE: there doesn't seem to be anything to check that the validator being slashed isn't the proposer of the block that contains the ps
+        // though it makes sense that a validator wouldn't proposer to slash itself!
+        // assert slashed_index != whistleblower_index;
+
+        var whistleblower_reward : Gwei := (s'.validators[slashed_index].effective_balance as int / WHISTLEBLOWER_REWARD_QUOTIENT as nat) as Gwei;
+        var proposer_reward := (whistleblower_reward as int / PROPOSER_REWARD_QUOTIENT as int) as Gwei;
+        var validator_penalty := (s'.validators[slashed_index].effective_balance as int / MIN_SLASHING_PENALTY_QUOTIENT as nat) as Gwei;
+
+        //s' := increase_balance(s', proposer_index, proposer_reward);
+        //s' := increase_balance(s', whistleblower_index, Gwei(whistleblower_reward - proposer_reward));
+        
+        //var validator := s'.validators[slashed_index];
+        // validator.slashed = True
+        // validator.withdrawable_epoch = max(validator.withdrawable_epoch, Epoch(epoch + EPOCHS_PER_SLASHINGS_VECTOR))
+        // state.slashings[epoch % EPOCHS_PER_SLASHINGS_VECTOR] += validator.effective_balance
+
+        assume (s'.slashings[epoch as int % EPOCHS_PER_SLASHINGS_VECTOR as nat] as int + s'.validators[slashed_index].effective_balance as int) < 0x10000000000000000;
+        assert slashed_index as int < |s'.balances|; 
+        assert proposer_index as int < |s'.balances|; 
+        assert whistleblower_index as int < |s'.balances|; 
+        assume s'.balances[proposer_index] as int + proposer_reward as int < 0x10000000000000000;
+        // Note: if proposer_index == whistleblower_index then the following assume statement is required rather than
+        // assume s'.balances[whistleblower_index] as int + (whistleblower_reward - proposer_reward) as int < 0x10000000000000000;
+        // The following assume statement covers both cases and will be replaced at a later date by functionality that
+        // takes into account the total amount of Eth available.
+        assume s'.balances[whistleblower_index] as int + whistleblower_reward  as int < 0x10000000000000000;
+
+        s'.(validators := s'.validators[slashed_index := s'.validators[slashed_index].(slashed := true,
+                                                            withdrawable_epoch := max(s'.validators[slashed_index].withdrawable_epoch as nat,(epoch as nat + EPOCHS_PER_SLASHINGS_VECTOR as nat)) as Epoch)],
+            slashings := s'.slashings[(epoch as int % EPOCHS_PER_SLASHINGS_VECTOR as nat) := s'.slashings[epoch as int % EPOCHS_PER_SLASHINGS_VECTOR as nat] + s'.validators[slashed_index].effective_balance],
+            balances := increase_balance(
+                            increase_balance(
+                                decrease_balance(s', slashed_index, validator_penalty), 
+                                proposer_index, 
+                                proposer_reward), 
+                            whistleblower_index, 
+                            (whistleblower_reward - proposer_reward)).balances)
+            
+        
+        // the triple nested mutation of balances is somewhat messy but for the moment it allows slashed_validator to remain as a function method 
+        //(rather than a method)
+
+    }
+
+     // Beacon State Mutators
+
+/** increase_balance
+     *  Increase the validator balance at index ``index`` by ``delta``.
+     *
+     *  @notes  The datatype Gwei has temporarily been changed from uint64 to nat so as to simplify the
+     *          properties required to process a deposit. Hence a further requires will be needed to prevent
+     *          overflow once this temporary simplification is removed.
+     *  
+     **/
+    // function method increase_balance(s: BeaconState, index: ValidatorIndex, delta: Gwei): BeaconState 
+    //     requires index as int < |s.balances| 
+    //     requires s.balances[index] as int + delta as int < 0x10000000000000000
+    //     ensures |s.balances| == |increase_balance(s,index,delta).balances|
+    //     ensures increase_balance(s,index,delta).balances[index] == s.balances[index] + delta
+    // {
+    //     s.(
+    //         balances := s.balances[index as int := (s.balances[index] + delta)]
+    //     )
+    // }
+
+    /** increase_balance
+     *  Increase the validator balance at index ``index`` by ``delta``.
+     *  
+     **/
+    function method increase_balance(s: BeaconState, index: ValidatorIndex, delta: Gwei): BeaconState 
+        requires index as int < |s.balances| 
+        requires s.balances[index] as int + delta as int < 0x10000000000000000
+        ensures |s.balances| == |increase_balance(s,index,delta).balances|
+        ensures increase_balance(s,index,delta).balances[index] == s.balances[index] + delta
+    {
+        s.(
+            balances := s.balances[index as int := (s.balances[index] + delta)]
+        )
+    }
+
+    /** decrease_balance
+     *  Decrease the validator balance at index ``index`` by ``delta``.
+     *
+     **/
+    function method decrease_balance(s: BeaconState, index: ValidatorIndex, delta: Gwei): BeaconState 
+        requires index as int < |s.balances| 
+        ensures |s.balances| == |decrease_balance(s,index,delta).balances|
+        ensures if s.balances[index] > delta then decrease_balance(s,index,delta).balances[index] == s.balances[index] - delta
+                else decrease_balance(s,index,delta).balances[index] == 0
+        ensures s.validators == decrease_balance(s,index,delta).validators
+    {
+        if s.balances[index] > delta then
+            s.(
+                balances := s.balances[index as int := (s.balances[index] - delta)]
+            )
+        else
+            s.(
+                balances := s.balances[index as int := 0]
+            )
+    }
+
+
+    function total_deposits(deposits: seq<Deposit>): nat
+    {
+        if |deposits| == 0 then 0
+        //else deposits[0].data.amount as nat + total_deposits(deposits[1..])
+        else total_deposits(deposits[..|deposits|-1]) + deposits[|deposits|-1].data.amount as nat
+    }
+
+    function total_balances(bal: seq<Gwei>): nat
+    {
+        if |bal| == 0 then 0
+        else bal[0] as nat + total_balances(bal[1..])
+    }
+
+
+    lemma slash_validator_lemma(s: BeaconState, slashed_index: ValidatorIndex, whistleblower_index: ValidatorIndex)
+        requires slashed_index as int < |s.validators| 
+        requires whistleblower_index as int < |s.validators| 
+        requires |s.validators| == |s.balances|
+        //requires s.validators[slashed_index].exitEpoch == FAR_FUTURE_EPOCH
+        requires |get_active_validator_indices(s.validators, get_current_epoch(s))| > 0
+        ensures slash_validator(s, slashed_index, whistleblower_index).validators[slashed_index].slashed
+    {
+
+    }
+
+
+    lemma slashValidatorPreservesMinimumActiveValidators(s: BeaconState, slashed_index: ValidatorIndex, whistleblower_index: ValidatorIndex)
+        requires slashed_index as int < |s.validators| 
+        requires whistleblower_index as int < |s.validators| 
+        requires |s.validators| == |s.balances|
+        //requires |get_active_validator_indices(s.validators, get_current_epoch(s))| > 0
+        requires minimumActiveValidators(s)
+        
+        ensures minimumActiveValidators(slash_validator(s,slashed_index,whistleblower_index))
+    {
+        slashValidatorPreservesActiveValidators(s, slashed_index, whistleblower_index);
+    }
+
+    // ?? prove that the only way slashed is set to true is by calling slash_validator?? 
+    
+    lemma slashValidatorPreservesActiveValidators(s: BeaconState, slashed_index: ValidatorIndex, whistleblower_index: ValidatorIndex)
+        requires slashed_index as int < |s.validators| 
+        requires whistleblower_index as int < |s.validators| 
+        requires |s.validators| == |s.balances|
+        //requires s.validators[slashed_index].exitEpoch == FAR_FUTURE_EPOCH
+        requires |get_active_validator_indices(s.validators, get_current_epoch(s))| > 0
+        
+        ensures get_active_validator_indices(s.validators, get_current_epoch(s)) ==
+                    get_active_validator_indices(slash_validator(s,slashed_index,whistleblower_index).validators, get_current_epoch(s))
+    {
+        
+        var epoch : Epoch := get_current_epoch(s);
+        var proposer_index := get_beacon_proposer_index(s);
+        var s' := initiate_validator_exit(s, slashed_index); // only validator exitEpoch & withdrawable_epoch fields possibly changed
+
+        // show initiate validator exit doesn't change the set of active validator indices
+        
+        assert |s.balances| == |s'.balances|;
+        assert |s'.balances| == |s'.validators|;
+        assert epoch == get_current_epoch(s');
+        
+        //assert initiate_validator_exit(s,slashed_index).validators[slashed_index].exitEpoch > epoch + MAX_SEED_LOOKAHEAD;
+        assert forall i :: (0 <= i < |s.validators|) && (i != slashed_index as int) ==> 
+                initiate_validator_exit(s,slashed_index).validators[i].exitEpoch == s.validators[i].exitEpoch;
+        
+        //assert s'.validators[slashed_index].exitEpoch > epoch + MAX_SEED_LOOKAHEAD;
+        assert forall i :: (0 <= i < |s.validators|) && (i != slashed_index as int) ==> 
+                s'.validators[i].exitEpoch == s.validators[i].exitEpoch;
+        
+        assert forall i :: (0 <= i < |s'.validators|) ==> 
+                is_active_validator(s.validators[i], epoch) == is_active_validator(s'.validators[i], epoch);
+
+        initiateValidatorExitPreservesActivateValidators(s.validators, s'.validators, epoch);
+        assert get_active_validator_indices(s'.validators, epoch) == get_active_validator_indices(s.validators, epoch);
+        assert |get_active_validator_indices(s'.validators, epoch)| > 0;
+
+        // show update to s', including rewards/penalties, doesn't change the set of active validator indices
+        var whistleblower_reward : Gwei := (s'.validators[slashed_index].effective_balance as int / WHISTLEBLOWER_REWARD_QUOTIENT as nat) as Gwei;
+        var proposer_reward := (whistleblower_reward as int / PROPOSER_REWARD_QUOTIENT as int) as Gwei;
+        var validator_penalty := (s'.validators[slashed_index].effective_balance as int / MIN_SLASHING_PENALTY_QUOTIENT as nat) as Gwei;
+
+        assume (s'.slashings[epoch as int % EPOCHS_PER_SLASHINGS_VECTOR as nat] as int + s'.validators[slashed_index].effective_balance as int) < 0x10000000000000000;
+        assert slashed_index as int < |s'.balances|; 
+        assert proposer_index as int < |s'.balances|; 
+        assert whistleblower_index as int < |s'.balances|; 
+        
+        assume s'.balances[proposer_index] as int + proposer_reward as int < 0x10000000000000000;
+        assume s'.balances[whistleblower_index] as int + whistleblower_reward  as int < 0x10000000000000000;
+
+
+        s' := s'.(  validators := s'.validators[slashed_index := s'.validators[slashed_index].(slashed := true,
+                                                            withdrawable_epoch := max(s'.validators[slashed_index].withdrawable_epoch as nat,(epoch as nat + EPOCHS_PER_SLASHINGS_VECTOR as nat)) as Epoch)],
+                    slashings := s'.slashings[(epoch as int % EPOCHS_PER_SLASHINGS_VECTOR as nat) := s'.slashings[epoch as int % EPOCHS_PER_SLASHINGS_VECTOR as nat] + s'.validators[slashed_index].effective_balance],
+                    balances := increase_balance(
+                                    increase_balance(
+                                        decrease_balance(s', slashed_index, validator_penalty), 
+                                        proposer_index, 
+                                        proposer_reward), 
+                                    whistleblower_index, 
+                                    (whistleblower_reward - proposer_reward)).balances);
+        
+        //assert s'.validators[slashed_index].exitEpoch > epoch + MAX_SEED_LOOKAHEAD;
+        assert forall i :: (0 <= i < |s.validators|) && (i != slashed_index as int) ==> 
+                s'.validators[i].exitEpoch == s.validators[i].exitEpoch;
+
+        assert forall i :: (0 <= i < |s'.validators|) ==> 
+                is_active_validator(s.validators[i], epoch) == is_active_validator(s'.validators[i], epoch);
+
+        assert s' == slash_validator(s,slashed_index,whistleblower_index);
+        
+        sameActiveValidatorsImpliesSameActiveValidatorIndices(s.validators, s'.validators, epoch);
+        assert get_active_validator_indices(s'.validators, epoch) == get_active_validator_indices(s.validators, epoch);
+    }
+
+    // is_valid_indexed_attestation
+    // Check if ``indexed_attestation`` is not empty, has sorted and unique indices and has a valid aggregate signature.
+    // Note: at this time only the first part of the check is being implemented
+
+    lemma valid_indexed_attestation_lemma(s: BeaconState, s': BeaconState, indexed_attestation: IndexedAttestation)
+        requires is_valid_indexed_attestation(s,indexed_attestation) 
+        ensures is_valid_indexed_attestation(s',indexed_attestation)
+    {
+        // Thanks Dafny
+    }
+
+    lemma initiateValidatorExitPreservesActivateValidators(sv: ListOfValidators, sv': ListOfValidators, epoch: Epoch)
+        requires |sv| == |sv'|
+        requires forall i :: (0 <= i < |sv'|) ==> 
+                is_active_validator(sv[i], epoch) == is_active_validator(sv'[i], epoch)
+        ensures get_active_validator_indices(sv', epoch) == get_active_validator_indices(sv, epoch)
+    {
+        if |sv'| == 0 {
+            assert get_active_validator_indices(sv', epoch) == get_active_validator_indices(sv, epoch);
+        }
+        else {
+            assert get_active_validator_indices(sv', epoch) == 
+                if is_active_validator(sv'[|sv'|-1], epoch) then 
+                    get_active_validator_indices(sv'[..|sv'|-1], epoch) + [(|sv'|-1) as ValidatorIndex]
+                else 
+                    get_active_validator_indices(sv'[..|sv'|-1], epoch);
+            
+            assert get_active_validator_indices(sv', epoch) == 
+                if is_active_validator(sv[|sv|-1], epoch) then 
+                    get_active_validator_indices(sv'[..|sv'|-1], epoch) + [(|sv'|-1) as ValidatorIndex]
+                else 
+                    get_active_validator_indices(sv'[..|sv'|-1], epoch);
+
+            assert |sv| == |sv'|;
+            assert get_active_validator_indices(sv', epoch) == 
+                if is_active_validator(sv[|sv|-1], epoch) then 
+                    get_active_validator_indices(sv'[..|sv|-1], epoch) + [(|sv|-1) as ValidatorIndex]
+                else 
+                    get_active_validator_indices(sv'[..|sv|-1], epoch);
+            initiateValidatorExitPreservesActivateValidators(sv[..|sv|-1], sv'[..|sv|-1], epoch);
+        }
+    }
+
+    
+    lemma sameActiveValidatorsImpliesSameActiveValidatorIndices(sv1: ListOfValidators, sv2: ListOfValidators, epoch: Epoch)
+        requires |sv1| == |sv2|   
+        requires forall i :: (0 <= i < |sv1|) ==> is_active_validator(sv1[i], epoch) == is_active_validator(sv2[i], epoch)
+        ensures get_active_validator_indices(sv1, epoch) == get_active_validator_indices(sv2, epoch)
+    {
+        if |sv1| == 0 {
+            assert get_active_validator_indices(sv2, epoch) == get_active_validator_indices(sv1, epoch);
+        }
+        else {
+            sameActiveValidatorsImpliesSameActiveValidatorIndices(sv1[..|sv1|-1], sv2[..|sv2|-1], epoch);
+        }
+    }
+
+
+    lemma individualBalanceBoundMaintained(sb: seq<Gwei>, d: Deposit)
+        requires total_balances(sb) + d.data.amount as int < 0x10000000000000000
+        ensures forall i :: 0 <= i < |sb| ==> sb[i] as int + d.data.amount as int < 0x10000000000000000
+    {
+        if |sb| == 0 {
+            // Thanks Dafny
+        }
+        else {
+            assert total_balances(sb) == sb[0] as int + total_balances(sb[1..]);
+            assert sb[0] as int + d.data.amount as int < 0x10000000000000000;
+            assert total_balances(sb[1..]) + d.data.amount as int < 0x10000000000000000;
+            individualBalanceBoundMaintained(sb[1..],d);
+        }
+    } 
+
+    
+
+
+    
+    lemma updateExistingBalance(s: BeaconState, index: ValidatorIndex, delta: Gwei)
+        requires index as int < |s.balances| 
+        requires s.balances[index] as int + delta as int < 0x10000000000000000
+        requires |s.balances| < VALIDATOR_REGISTRY_LIMIT as int
+
+        ensures total_balances(increase_balance(s,index,delta).balances) == total_balances(s.balances) + delta as int
+    {
+        //assert increase_balance(s,index,delta).balances[index] == s.balances[index] + delta;
+        //assert forall i :: 0 <= i < |s.balances| && i != index as int ==> increase_balance(s,index,delta).balances[i] == s.balances[i];
+
+        if index as int < |s.balances|-1 {
+            assert increase_balance(s,index,delta).balances == increase_balance(s,index,delta).balances[..index] + [increase_balance(s,index,delta).balances[index]] + increase_balance(s,index,delta).balances[(index+1)..];
+                                                                
+            //assert total_balances(increase_balance(s,index,delta).balances[..index]) == total_balances(s.balances[..index]);
+            //assert total_balances([increase_balance(s,index,delta).balances[index]]) == total_balances([s.balances[index]]) + delta as int;
+            //assert total_balances(increase_balance(s,index,delta).balances[(index+1)..]) == total_balances(s.balances[(index+1)..]);
+
+            //assert total_balances(increase_balance(s,index,delta).balances) == total_balances(increase_balance(s,index,delta).balances[..index] + [increase_balance(s,index,delta).balances[index]] + increase_balance(s,index,delta).balances[(index+1)..]);
+
+            distBalancesProp(increase_balance(s,index,delta).balances[..index], [increase_balance(s,index,delta).balances[index]]);
+            //assert total_balances(increase_balance(s,index,delta).balances[..index] + [increase_balance(s,index,delta).balances[index]]) == total_balances(increase_balance(s,index,delta).balances[..index]) + total_balances([increase_balance(s,index,delta).balances[index]]);
+            distBalancesProp(increase_balance(s,index,delta).balances[..index]+[increase_balance(s,index,delta).balances[index]], increase_balance(s,index,delta).balances[(index+1)..]);
+            //assert total_balances(increase_balance(s,index,delta).balances[..index] + [increase_balance(s,index,delta).balances[index]] + increase_balance(s,index,delta).balances[(index+1)..]) == total_balances(increase_balance(s,index,delta).balances[..index]) + total_balances([increase_balance(s,index,delta).balances[index]]) + total_balances(increase_balance(s,index,delta).balances[index+1..]);
+
+            //assert total_balances(increase_balance(s,index,delta).balances) == total_balances(increase_balance(s,index,delta).balances[..index]) + total_balances([increase_balance(s,index,delta).balances[index]]) + total_balances(increase_balance(s,index,delta).balances[index+1..]);
+            //assert total_balances(increase_balance(s,index,delta).balances) == total_balances(s.balances[..index]) + total_balances([s.balances[index]]) + delta as int + total_balances(s.balances[(index+1)..]);
+
+            //assert total_balances(increase_balance(s,index,delta).balances) == total_balances(s.balances[..index]) + total_balances([s.balances[index]]) + total_balances(s.balances[(index+1)..]) + delta as int;
+
+            assert s.balances == s.balances[..index] + [s.balances[index]] + s.balances[(index+1)..];
+            //assert total_balances(s.balances) == total_balances(s.balances[..index] + [s.balances[index]] + s.balances[(index+1)..]);
+
+            distBalancesProp(s.balances[..index], [s.balances[index]]);
+            //assert total_balances(s.balances[..index] + [s.balances[index]]) == total_balances(s.balances[..index]) + total_balances([s.balances[index]]);
+            distBalancesProp(s.balances[..index]+[s.balances[index]], s.balances[(index+1)..]);
+            //assert total_balances(s.balances[..index] + [s.balances[index]] + s.balances[(index+1)..]) == total_balances(s.balances[..index]) + total_balances([s.balances[index]]) + total_balances(s.balances[index+1..]);
+
+            //assert total_balances(increase_balance(s,index,delta).balances) == total_balances(s.balances) + delta as int;
+        }
+        else {
+            //assert index as int == |s.balances| - 1;
+            assert increase_balance(s,index,delta).balances == increase_balance(s,index,delta).balances[..index] + [increase_balance(s,index,delta).balances[index]];
+                                                                
+            //assert total_balances(increase_balance(s,index,delta).balances[..index]) == total_balances(s.balances[..index]);
+            //assert total_balances([increase_balance(s,index,delta).balances[index]]) == total_balances([s.balances[index]]) + delta as int;
+            
+            //assert total_balances(increase_balance(s,index,delta).balances) == total_balances(increase_balance(s,index,delta).balances[..index] + [increase_balance(s,index,delta).balances[index]]);
+
+            distBalancesProp(increase_balance(s,index,delta).balances[..index], [increase_balance(s,index,delta).balances[index]]);
+            //assert total_balances(increase_balance(s,index,delta).balances[..index] + [increase_balance(s,index,delta).balances[index]]) == total_balances(increase_balance(s,index,delta).balances[..index]) + total_balances([increase_balance(s,index,delta).balances[index]]);
+            
+            
+            //assert total_balances(increase_balance(s,index,delta).balances) == total_balances(s.balances[..index]) + total_balances([s.balances[index]]) + delta as int;
+
+            assert s.balances == s.balances[..index] + [s.balances[index]] ;
+            //assert total_balances(s.balances) == total_balances(s.balances[..index] + [s.balances[index]]);
+
+            distBalancesProp(s.balances[..index], [s.balances[index]]);
+            //assert total_balances(s.balances[..index] + [s.balances[index]]) == total_balances(s.balances[..index]) + total_balances([s.balances[index]]);
+            
+            //assert total_balances(increase_balance(s,index,delta).balances) == total_balances(s.balances) + delta as int;
+        }
+    }
+
+    lemma distBalancesProp(sb1: seq<Gwei>, sb2: seq<Gwei>)
+        ensures total_balances(sb1 + sb2) == total_balances(sb1) + total_balances(sb2) 
+    {
+        if |sb1| == 0 {
+            assert sb1 + sb2 == sb2;
+        }
+        else {
+            var sb := sb1 + sb2;
+            //assert sb == [sb1[0]] +  sb1[1..] + sb2;
+            assert sb[1..] == sb1[1..] + sb2;
+            assert total_balances(sb) == sb[0] as int + total_balances(sb[1..]);
+            //assert total_balances(sb1 + sb2) == sb[0] as int + total_balances(sb1[1..] + sb2);
+            distBalancesProp(sb1[1..],sb2);
+
+        }
+    }
+
+    lemma distDepositsProp(sd1: seq<Deposit>, sd2: seq<Deposit>)
+        ensures total_deposits(sd1 + sd2) == total_deposits(sd1) + total_deposits(sd2) 
+    {
+        if |sd2| == 0 {
+            assert sd1 + sd2 == sd1;
+        }
+        else {
+            var sd := sd1 + sd2;
+            //assert sd == sd1 + sd2[..|sd2|-1] +  [sd2[|sd2|-1]];
+            assert sd[..|sd|-1] == sd1 + sd2[..|sd2|-1] ;
+            assert total_deposits(sd) == total_deposits(sd[..|sd|-1]) + sd2[|sd2|-1].data.amount as int;
+            //assert total_deposits(sd1 + sd2) == total_deposits(sd1 + sd2[..|sd2|-1] ) + sd2[|sd2|-1].data.amount as int;
+            distDepositsProp(sd1, sd2[..|sd2|-1] );
+        }
+    }
+    lemma subsetDepositSumProp(deposits: seq<Deposit>, i: nat)
+        requires i <= |deposits|
+        ensures total_deposits(deposits[..i]) <= total_deposits(deposits);
+    {
+        if i == |deposits| {
+            assert deposits[..i] == deposits;
+        }
+        else {
+            //assert i < |deposits|;
+            assert deposits == deposits[..i] + deposits[i..];
+            assert total_deposits(deposits) == total_deposits(deposits[..i] + deposits[i..]);
+            distDepositsProp(deposits[..i], deposits[i..]);
+            //assert total_deposits(deposits[..i] + deposits[i..]) == total_deposits(deposits[..i]) + total_deposits(deposits[i..]); 
+        }
+    }
+
+
+    // function method  get_total_balance(state: BeaconState, indices: set<ValidatorIndex>) : Gwei
+    // """
+    // Return the combined effective balance of the ``indices``.
+    // ``EFFECTIVE_BALANCE_INCREMENT`` Gwei minimum to avoid divisions by zero.
+    // Math safe up to ~10B ETH, afterwhich this overflows uint64.
+    // """
+    // {
+        // return Gwei(max(EFFECTIVE_BALANCE_INCREMENT, sum([state.validators[index].effective_balance for index in indices])));
+        //  for now we return the size of indices
+        // |indices| as Gwei 
+    // }
+
+
+    function method get_total_balance_seq(s: BeaconState, indices: seq<ValidatorIndex>) : Gwei
+        requires forall i :: 0 <= i < |indices| ==> indices[i] as nat < |s.validators|
+        ensures EFFECTIVE_BALANCE_INCREMENT <= get_total_balance_seq(s, indices)
+
+    {
+        max(EFFECTIVE_BALANCE_INCREMENT as nat, get_total_balance_seq_helper(s, indices) as nat) as Gwei
+    }
+
+    function method get_total_balance_seq_helper(s: BeaconState, indices: seq<ValidatorIndex>) : Gwei
+        requires forall i :: 0 <= i < |indices| ==> indices[i] as nat < |s.validators|
+    {
+        if |indices| == 0 then 0 as Gwei
+        else
+            assume s.validators[indices[0]].effective_balance as nat + get_total_balance_seq_helper(s, indices[1..]) as nat < 0x10000000000000000;
+            s.validators[indices[0]].effective_balance + get_total_balance_seq_helper(s, indices[1..]) 
+    }
+
+    function method get_total_balance(s: BeaconState, indices: set<ValidatorIndex>) : Gwei
+        requires forall i : ValidatorIndex :: i in indices ==> i as nat < |s.validators|
+
+    {
+        max(EFFECTIVE_BALANCE_INCREMENT as nat, get_total_balance_helper(s, indices) as nat) as Gwei
+    }
+
+    function method get_total_balance_helper(s: BeaconState, indices: set<ValidatorIndex>) : Gwei
+        requires forall i : ValidatorIndex :: i in indices ==> i as nat < |s.validators|
+    {
+        if |indices| == 0 then 0 as Gwei
+        else
+            var y := PickIndex(indices);
+            assume s.validators[y].effective_balance as nat + get_total_balance_helper(s, indices - {y}) as nat < 0x10000000000000000;
+            s.validators[y].effective_balance + get_total_balance_helper(s, indices - {y}) 
+    }
+
+    function method PickIndex(s: set<ValidatorIndex>): ValidatorIndex
+        requires s != {}
+    {
+        HasMinimum(s);
+        var z :| z in s && forall y :: y in s ==> z as nat <= y as nat;
+        z
+    }
+
+    lemma HasMinimum(s: set<ValidatorIndex>)
+        requires s != {}
+        ensures exists z :: z in s && forall y :: y in s ==> z <= y
+        // Ref: https://stackoverflow.com/questions/51207795/the-hilbert-epsilon-operator
+    {
+        var z :| z in s;
+        if s == {z} {
+            // the mimimum of a singleton set is its only element
+        } else if forall y :: y in s ==> z <= y {
+            // we happened to pick the minimum of s
+        } else {
+            // s-{z} is a smaller, nonempty set and it has a minimum
+            var s' := s - {z};
+            HasMinimum(s');
+            var z' :| z' in s' && forall y :: y in s' ==> z' <= y;
+            // the minimum of s' is the same as the miminum of s
+            forall y | y in s
+            ensures z' <= y
+            {
+            if
+            case y in s' =>
+                assert z' <= y;  // because z' in minimum in s'
+            case y == z =>
+                var k :| k in s && k < z;  // because z is not minimum in s
+                assert k in s';  // because k != z
+            }
+        }
+    }
+
+    function method get_total_active_balance(state: BeaconState) : Gwei
+        // requires |state.validators| < 0x10000000000000000
+    // """
+    // Return the combined effective balance of the active validators.
+    // Note: ``get_total_balance`` returns ``EFFECTIVE_BALANCE_INCREMENT`` Gwei minimum to avoid divisions by zero.
+    // """
+    {
+        // get_total_balance(state, set(get_active_validator_indices(state, get_current_epoch(state))))
+        assert(|state.validators| < 0x10000000000000000);
+        |state.validators| as uint64
+    }
+
+    function method get_total_active_balance_full(s: BeaconState) : Gwei
+        // requires |state.validators| < 0x10000000000000000
+        ensures EFFECTIVE_BALANCE_INCREMENT <= get_total_active_balance_full(s) 
+    // """
+    // Return the combined effective balance of the active validators.
+    // Note: ``get_total_balance`` returns ``EFFECTIVE_BALANCE_INCREMENT`` Gwei minimum to avoid divisions by zero.
+    // """
+    {
+        get_total_balance_seq(s, get_active_validator_indices(s.validators, get_current_epoch(s)))
+    }
+
+/**
+     *  The number of attestations for a pair of checkpoints.
+     *  
+     *  @param  xa  The known list of attestations (votes).
+     *  @param  src A checkpoint.
+     *  @param  tgt A checkpoint.
+     *  @returns    The number of votes for src --> tgt in `xa`.
+     */
+    function method countAttestationsForLink(xa : seq<PendingAttestation>, src : CheckPoint, tgt: CheckPoint) : nat
+        ensures countAttestationsForLink(xa, src, tgt) <= |xa|
+        decreases xa
+    {
+        if |xa| == 0 then 
+            0
+        else 
+            (if xa[0].data.source == src && xa[0].data.target == tgt then 
+                1
+
+            else 
+                0
+            ) + countAttestationsForLink(xa[1..], src, tgt)
+    }
+
+    /**
+     *  Collect set of indices of validators attesting a link.
+     *
+     *  @param  xa      A seq of attestations.
+     *  @param  src     The source checkpoint of the link.
+     *  @param  tgt     The target checkpoint of the link.
+     *  @returns        The set of validators's indices that vote for (src. tgt) in `xa`. 
+     */
+     function collectValidatorsAttestatingForLink(xa : seq<PendingAttestation>, src : CheckPoint, tgt: CheckPoint) : set<nat>
+        ensures forall e :: e in collectValidatorsAttestatingForLink(xa, src, tgt) ==>
+            e < MAX_VALIDATORS_PER_COMMITTEE as nat
+        ensures |collectValidatorsAttestatingForLink(xa, src, tgt)| <= MAX_VALIDATORS_PER_COMMITTEE as nat
+        decreases xa
+    {
+        if |xa| == 0 then 
+            { }
+        else 
+            unionCardBound(trueBitsCount(xa[0].aggregation_bits),
+                collectValidatorsAttestatingForLink(xa[1..], src, tgt), MAX_VALIDATORS_PER_COMMITTEE as nat);
+            (if xa[0].data.source == src && xa[0].data.target == tgt then 
+                trueBitsCount(xa[0].aggregation_bits)
+            else 
+                {}
+            ) + collectValidatorsAttestatingForLink(xa[1..], src, tgt)
+    }
+
+    /**
+     *  Collect set of indices of validators attesting a link to a given target.
+     *
+     *  @param  xa      A seq of attestations.
+     *  @param  tgt     The target checkpoint of the link.
+     *  @returns        The set of validators's indices that vote for (_. tgt) in `xa`. 
+     */
+    function collectValidatorsIndicesAttestatingForTarget(xa : seq<PendingAttestation>, tgt: CheckPoint) : set<nat>
+        ensures forall e :: e in collectValidatorsIndicesAttestatingForTarget(xa, tgt) ==>
+            e < MAX_VALIDATORS_PER_COMMITTEE as nat
+        ensures |collectValidatorsIndicesAttestatingForTarget(xa, tgt)| <= MAX_VALIDATORS_PER_COMMITTEE as nat
+        decreases xa
+    {
+        if |xa| == 0 then 
+            { }
+        else 
+            unionCardBound(trueBitsCount(xa[0].aggregation_bits),
+                collectValidatorsIndicesAttestatingForTarget(xa[1..], tgt), MAX_VALIDATORS_PER_COMMITTEE as nat);
+            (if xa[0].data.target == tgt then 
+                trueBitsCount(xa[0].aggregation_bits)
+            else 
+                {}
+            ) + collectValidatorsIndicesAttestatingForTarget(xa[1..], tgt)
+    }
+
+    /**
+     *  Collect the set of indices for which xb[i] is true.
+     *  
+     *  @param  xb  A sequence of bools.
+     *  @returns    The number of elements that are true in `xb`.
+     */
+    function trueBitsCount(xb : seq<bool>) : set<nat> 
+        ensures |trueBitsCount(xb)| <= |xb|
+        ensures forall i :: i in trueBitsCount(xb) <==> 0 <= i < |xb| && xb[i]
+        decreases xb
+    {
+        if |xb| == 0 then 
+            {}
+        else 
+            (if xb[|xb| - 1] then { |xb| - 1 } else {}) + trueBitsCount(xb[..|xb| - 1])
+    }
+
+    /**
+     *  The set of validators attesting to a target is larger than the set 
+     *  of validators attesting to a link with that target. 
+     *
+     *  @param  xa      A seq of attestations.
+     *  @param  src     The source checkpoint of the link.
+     *  @param  tgt     The target checkpoint of the link.
+     */
+    lemma {:induction xa} attForTgtLargerThanLinks(xa : seq<PendingAttestation>, src : CheckPoint, tgt: CheckPoint)
+        ensures collectValidatorsAttestatingForLink(xa, src, tgt) <= collectValidatorsIndicesAttestatingForTarget(xa, tgt) 
+        ensures |collectValidatorsAttestatingForLink(xa, src, tgt)| <= |collectValidatorsIndicesAttestatingForTarget(xa, tgt)| 
+    {
+        assert(collectValidatorsAttestatingForLink(xa, src, tgt) <= collectValidatorsIndicesAttestatingForTarget(xa, tgt) );
+        cardIsMonotonic(collectValidatorsAttestatingForLink(xa, src, tgt), collectValidatorsIndicesAttestatingForTarget(xa, tgt));
+    }
+
+    /**
+     *  @param  state   A beacon state.
+     *  @param  epoch   An epoch which is either the state's epoch ior the previous one.
+     *  @returns        The current (resp. previous) list of attestations if epoch is 
+     *                  state's epoch (resp. epoch before state's epoch). 
+     *  @note           The function name is misleading as it seems to be a counter-part
+     *                  or symmetric of `get_matching_target_attestations` but it is not.
+     *                  Moreover it does not perform any matching as the name indicates,
+     *                  and the matching/filtering is done in `get_matching_target_attestations`.
+     *                  A better name may be `get_attestations_at_epoch`.
+     *  @note           An even better solution would be to remove this function 
+     *                  and directly `use state.current_epoch_attestations` or 
+     *                  `state.previous_epoch_attestations` in the callers.
+     */
+    function method get_matching_source_attestations(state: BeaconState, epoch: Epoch) : seq<PendingAttestation>
+        //  report? -> meaning of i in (a, b)? seems to be closed interval ...
+        requires get_previous_epoch(state) <= epoch <= get_current_epoch(state)
+        ensures |get_matching_source_attestations(state, epoch)| < 0x10000000000000000
+
+        // this property will be assumed for the moment
+        //ensures forall i :: 0 <= i < |get_matching_source_attestations(state, epoch)| 
+        //    ==> get_matching_source_attestations(state, epoch)[i].data.index 
+        //        < get_committee_count_per_slot(state, compute_epoch_at_slot(get_matching_source_attestations(state, epoch)[i].data.slot)) <= TWO_UP_6
+    {
+        // assert epoch in (get_previous_epoch(state), get_current_epoch(state))
+        // return state.current_epoch_attestations if epoch == get_current_epoch(state) else state.previous_epoch_attestations
+        if epoch == get_current_epoch(state) then
+            state.current_epoch_attestations
+        else 
+            state.previous_epoch_attestations
+    }  
+
+    /**
+     *  @param  state   A beacon state.
+     *  @param  epoch   An epoch which is either the state's epoch or the previous one.
+     *  @returns        Attestations at epoch with a target that is the block root
+     *                  recorded for that epoch.         
+     *
+     *  @note           This function does not check the epoch of the source attestation.
+     *                  As a result if the seq of attestations in   
+     *                  `state.previous/current_epoch_attestations` contains the same 
+     *                  block root at different epochs, all the attestations will be collect.
+     *                  However the following note seems to suggest that this cannot happen.
+     *
+     *  @note           From the eth2.0 specs: When processing attestations, we already only *                  accept attestations that have the correct Casper FFG source checkpoint 
+     *                  (specifically, the most recent justified checkpoint that the chain 
+     *                  knows about). The goal of this function is to get all attestations 
+     *                  that have a correct Casper FFG source. Hence, it can safely just 
+     *                  return all the PendingAttestations for the desired epoch 
+     *                  (current or previous).
+     *  @note           The claim "it can safely just return all the PendingAttestations for 
+     *                  the desired epoch (current or previous)." is valid only if all the 
+     *                  attestations in `state.previous/current_epoch_attestations`
+     *                  are well-formed. 
+     *  @todo           We should add this constraint to the pre-conditions of this function.
+     */
+    function method get_matching_target_attestations(state: BeaconState, epoch: Epoch) : seq<PendingAttestation>
+        requires epoch as nat *  SLOTS_PER_EPOCH as nat  <  state.slot as nat
+        requires state.slot - epoch *  SLOTS_PER_EPOCH <=  SLOTS_PER_HISTORICAL_ROOT 
+        requires 1 <= get_previous_epoch(state) <= epoch <= get_current_epoch(state)
+        // requires 
+
+        ensures |get_matching_target_attestations(state, epoch)| < 0x10000000000000000
+        ensures forall a :: a in get_matching_target_attestations(state, epoch) ==>
+                    a.data.target.root == get_block_root(state, epoch)
+
+        ensures var e := get_previous_epoch(state);
+            epoch == e ==> 
+                get_matching_target_attestations(state, e) == 
+                filterAttestations(state.previous_epoch_attestations, get_block_root(state, e))
+        ensures var e := get_current_epoch(state);
+            epoch == e ==> 
+                get_matching_target_attestations(state, e) == 
+                filterAttestations(state.current_epoch_attestations, get_block_root(state, e))
+        decreases epoch //  seems needed to prove last two post-conds
+    {
+        //  Get attestattions at epoch as recorded in state (previous epoch or current epoch).
+        var ax := get_matching_source_attestations(state, epoch);
+        //  Collect attestations for (i.e. with target equal to) block root at epoch
+        filterAttestations(ax, get_block_root(state, epoch))
+    }
+
+    function method get_matching_head_attestations(state: BeaconState, epoch: Epoch) : seq<PendingAttestation>
+        requires epoch as nat *  SLOTS_PER_EPOCH as nat  <  state.slot as nat
+        requires state.slot - epoch *  SLOTS_PER_EPOCH <=  SLOTS_PER_HISTORICAL_ROOT 
+        requires 1 <= get_previous_epoch(state) <= epoch <= get_current_epoch(state)
+        
+        ensures |get_matching_head_attestations(state, epoch)| < 0x10000000000000000
+        ensures forall a :: a in get_matching_head_attestations(state, epoch) ==>
+                    a.data.slot < state.slot &&
+                    state.slot - a.data.slot <= SLOTS_PER_HISTORICAL_ROOT &&
+                    a.data.beacon_block_root == get_block_root_at_slot(state, a.data.slot)
+
+    {
+        var ax := get_matching_target_attestations(state, epoch);
+        filterAttestationsyy(ax, state)
+    }
+    
+
+    function method get_attesting_balance(state: BeaconState, attestations: seq<PendingAttestation>) : Gwei 
+        requires |attestations| < 0x10000000000000000
+    // """
+    // Return the combined effective balance of the set of unslashed validators participating in ``attestations``.
+    // Note: ``get_total_balance`` returns ``EFFECTIVE_BALANCE_INCREMENT`` Gwei minimum to avoid divisions by zero.
+    // """
+    {
+        // get_total_balance(state, get_unslashed_attesting_indices(state, attestations))
+        |attestations| as Gwei 
+    }
+
+    function method get_unslashed_attesting_indices(s: BeaconState, attestations: seq<PendingAttestation>): set<ValidatorIndex>
+        //requires forall i :: 0 <= i < |attestations| ==> attestations[i].data.index < get_committee_count_per_slot(s, compute_epoch_at_slot(attestations[i].data.slot)) <= TWO_UP_6
+        requires forall a :: a in attestations ==> a.data.index < get_committee_count_per_slot(s, compute_epoch_at_slot(a.data.slot)) <= TWO_UP_6
+        requires forall a :: a in attestations ==> TWO_UP_5 as nat <= |get_active_validator_indices(s.validators, compute_epoch_at_slot(a.data.slot))| <= TWO_UP_11 as nat * TWO_UP_11 as nat 
+        requires forall a :: a in attestations ==> 0 < |get_beacon_committee(s, a.data.slot, a.data.index)| == |a.aggregation_bits| <= MAX_VALIDATORS_PER_COMMITTEE as nat 
+
+        ensures forall i  :: i in get_unslashed_attesting_indices(s, attestations) ==> i as nat < |s.validators|
+    {
+        if |attestations| == 0 then {}
+        else 
+            // output = set()  # type: Set[ValidatorIndex]
+            // for a in attestations:
+            //      output = output.union(get_attesting_indices(state, a.data, a.aggregation_bits))
+            //      return set(filter(lambda index: not state.validators[index].slashed, output))       
+            var indices := get_attesting_indices(s, attestations[0].data, attestations[0].aggregation_bits);
+            var unslashed_indices := unslashed_attesting_indices_helper(s,indices);
+            unslashed_indices + get_unslashed_attesting_indices(s, attestations[1..])
+    }
+    
+    function method unslashed_attesting_indices_helper(s: BeaconState, indices: set<ValidatorIndex>): set<ValidatorIndex>
+        requires forall i  :: i in indices ==> i as nat < |s.validators|
+        ensures forall i  :: i in unslashed_attesting_indices_helper(s, indices) ==> i as nat < |s.validators|
+    {
+       if indices == {} then {}
+       else 
+            var x := PickIndex(indices);
+            if !s.validators[x].slashed then {x} + unslashed_attesting_indices_helper(s, indices - {x})
+            else unslashed_attesting_indices_helper(s, indices - {x})
+    }
+
+
+    
+    // def get_attesting_indices(state: BeaconState,
+    //                       data: AttestationData,
+    //                       bits: Bitlist[MAX_VALIDATORS_PER_COMMITTEE]) -> Set[ValidatorIndex]:
+    // """
+    // Return the set of attesting indices corresponding to ``data`` and ``bits``.
+    // """
+    // committee = get_beacon_committee(state, data.slot, data.index)
+    // return set(index for i, index in enumerate(committee) if bits[i])
+    function method get_attesting_indices(s: BeaconState, data: AttestationData, bits: AggregationBits) : set<ValidatorIndex>
+        requires TWO_UP_5 as nat <= |get_active_validator_indices(s.validators, compute_epoch_at_slot(data.slot))| <= TWO_UP_11 as nat * TWO_UP_11 as nat 
+        requires data.index < get_committee_count_per_slot(s, compute_epoch_at_slot(data.slot)) <= TWO_UP_6
+        requires 0 < |get_beacon_committee(s, data.slot, data.index)| == |bits| <= MAX_VALIDATORS_PER_COMMITTEE as nat
+
+        ensures forall i :: i in get_attesting_indices(s, data, bits) ==> i as nat < |s.validators|
+    {
+        var committee := get_beacon_committee(s, data.slot, data.index);
+        assert |committee| <= |bits|;
+        assert forall e :: e in committee ==> e as nat < |s.validators|;
+        filterIndicesxx(committee, bits)
+
+    }
+
+    function method filterIndicesxx(sv : seq<ValidatorIndex>, bits: AggregationBits) : set<ValidatorIndex>
+        requires |sv| <= |bits|
+        ensures |filterIndicesxx(sv, bits)| <= |sv|
+        ensures forall i :: 0 <= i < |sv| && bits[i] ==> sv[i] in filterIndicesxx(sv, bits)
+        ensures |filterIndicesxx(sv, bits)| <= |sv|
+        ensures forall i :: i in filterIndicesxx(sv, bits) ==> i in sv
+        decreases sv
+    {
+        if |sv| == 0 then 
+            {}
+        else 
+            (if bits[0] then {sv[0]} else {})
+                + filterIndicesxx(sv[1..], bits[1..])
+    }
+
+    /**
+     *  Collect attestations with a specific target.
+     *
+     *  @param  x   A list of attestations.
+     *  @param  br  A root value (hash of a block or block root). 
+     *  @returns    The subset of `xl` that corresponds to attestation with target `r`.
+     */
+    function method filterAttestations(xl : seq<PendingAttestation>, br : Root) : seq<PendingAttestation>
+        ensures |filterAttestations(xl, br)| <= |xl|
+        ensures forall a :: a in xl && a.data.target.root == br <==> a in filterAttestations(xl, br) 
+        decreases xl
+    {
+        if |xl| == 0 then 
+            []
+        else 
+            (if xl[0].data.target.root == br then [xl[0]] else [])
+                + filterAttestations(xl[1..], br)
+    }
+
+    function method filterAttestationsyy(xl : seq<PendingAttestation>, s : BeaconState) : seq<PendingAttestation>
+        ensures |filterAttestationsyy(xl, s)| <= |xl|
+        ensures forall a :: a in xl && 
+                            a.data.slot < s.slot &&
+                            s.slot - a.data.slot <= SLOTS_PER_HISTORICAL_ROOT &&
+                            a.data.beacon_block_root == get_block_root_at_slot(s, a.data.slot) <==> a in filterAttestationsyy(xl, s) 
+        decreases xl
+    {
+        if |xl| == 0 then 
+            []
+        else 
+            (if xl[0].data.slot < s.slot &&
+                s.slot - xl[0].data.slot <= SLOTS_PER_HISTORICAL_ROOT &&
+                xl[0].data.beacon_block_root == get_block_root_at_slot(s, xl[0].data.slot) then [xl[0]] else [])
+
+                + filterAttestationsyy(xl[1..], s)
+
+    }
+
+     ///////////////////////
+    predicate attestationIsWellFormed(s: BeaconState, a: Attestation)
+    {
+        get_previous_epoch(s) <= a.data.target.epoch <= get_current_epoch(s)  
+        /** Epoch of target matches epoch of the slot the attestation is made. */
+        && a.data.target.epoch == compute_epoch_at_slot(a.data.slot)
+        /** Attestation is not too old and not too recent. */
+        && a.data.slot as nat + MIN_ATTESTATION_INCLUSION_DELAY as nat <= s.slot as nat <= a.data.slot as nat + SLOTS_PER_EPOCH as nat
+        
+        && a.data.index < get_committee_count_per_slot(s, a.data.target.epoch)
+        // Preconditions for get_beacon_committee
+        && TWO_UP_5 as nat <= |get_active_validator_indices(s.validators, compute_epoch_at_slot(a.data.slot))| <= TWO_UP_11 as nat * TWO_UP_11 as nat 
+        && a.data.index < TWO_UP_6 // this comes from the assert on attestations in process_attestations
+        // same as above
+        //&& a.data.index < get_committee_count_per_slot(s, compute_epoch_at_slot(a.data.slot)) // at most 64 committees per slot 
+    
+        && |a.aggregation_bits| == |get_beacon_committee(s, a.data.slot, a.data.index)|
+        
+        && (if a.data.target.epoch == get_current_epoch(s) then  
+            a.data.source == s.current_justified_checkpoint
+           else 
+            a.data.source == s.previous_justified_checkpoint)
+
+    }
+
+    lemma AttestationHelperLemma(s: BeaconState, s1: BeaconState, a: Attestation)
+        requires attestationIsWellFormed(s, a);
+        requires s1.validators == s.validators
+        requires s1.slot == s.slot
+        requires s1.current_justified_checkpoint == s.current_justified_checkpoint
+        requires s1.previous_justified_checkpoint == s.previous_justified_checkpoint
+        ensures attestationIsWellFormed(s1, a);
+    { // Thanks Dafny
+    }
+
 
 }
