src/dafny/beacon/statetransition/ProcessOperations.s.dfy
@@ -20,9 +20,7 @@ include "../../utils/SeqHelpers.dfy"
 include "../../ssz/Constants.dfy"
 include "../BeaconChainTypes.dfy"
 include "../validators/Validators.dfy"
-include "../validators/ValidatorHelpers.dfy"
 include "../attestations/AttestationsTypes.dfy"
-include "../attestations/AttestationsHelpers.dfy"
 include "../Helpers.dfy"
 include "../Helpers.s.dfy"
 include "../../ssz/Serialise.dfy"
@@ -40,9 +38,7 @@ module ProcessOperationsSpec {
     import opened Constants
     import opened BeaconChainTypes
     import opened Validators
-    import opened ValidatorHelpers
     import opened AttestationsTypes
-    import opened AttestationsHelpers
     import opened BeaconHelpers
     import opened BeaconHelperSpec
     import opened MathHelpers
